---
title: "Data 605 HW14: Taylor Series Approximations"
author: "Sin Ying Wong"
date: "12/06/2020"
output:
  rmdformats::readthedown:
    code_folding: hide
    df_print: paged
    highlight: tango
    number_sections: yes
    smooth_scroll: yes
    theme: united
    toc_collapsed: yes
    toc_depth: 5
    toc_float: yes
  html_document:
    df_print: paged
    toc: yes
    toc_collapsed: yes
    toc_float: yes
  pdf_document:
    extra_dependencies:
    - geometry
    - multicol
    - multirow
  word_document:
    toc: yes
    toc_depth: '5'
theme: lumen
number_sections: yes
toc_depth: 3
---

```{r setup, include=FALSE}
knitr::opts_chunk$set(message = FALSE)
```

Please refer to the [Assignment 14 Document](https://github.com/shirley-wong/Data-605/blob/master/Assignment14/hw14.pdf).


# Problem Set

This week, we'll work out some Taylor Series expansions of popular functions.

- $f(x) = \frac{1}{(1-x)}$
- $f(x) = e^{x}$
- $f(x) = ln(1+x)$

For each function, only consider its valid ranges as indicated in the notes when you are computing the Taylor Series expansion. Please submit your assignment as a R-Markdown document.

# Taylor Series

![](https://github.com/shirley-wong/Data-605/blob/master/Assignment14/Taylor%20Series.PNG?raw=true)

# Answers

## Q1

$$f(x) = \frac{1}{(1-x)}$$

Taking derivatives, we have

$$f'(x) = (-1)(1-x)^{-2}(-1)=(1-x)^{-2}$$
$$f''(x) = (-2)(1-x)^{-3}(-1)=2(1-x)^{-3}$$
$$f'''(x) = (2)(-3)(1-x)^{-4}(-1) = 6(1-x)^{-4}$$
$$f''''(x) = (6)(-4)(1-x)^{-5}(-1) = 24(1-x)^{-5}$$

Evaluating the formula at $x=0$, we get

$$f(x) = \frac{1}{(1-x)}$$

$$= \sum_{n=0}^{\infty} \frac{f^{(n)}(0)}{n!}x^{n}$$
$$= f(0) + f'(0)x + f''(0)\frac{x^{2}}{2!} + f'''(0)\frac{x^{3}}{3!} + \cdots$$
$$= 1 + x + \frac{2}{2!}x^{2} + \frac{6}{3!}x^{3} + \frac{24}{4!}x^{4} + \cdots $$
$$= 1+x+x^{2}+x^{3}+x^{4}\cdots$$


## Q2

$$f(x) = e^{x}$$

Taking derivatives, we have

$$f'(x) = e^{x}$$
$$f''(x) = e^{x}$$
$$f'''(x) = e^{x}$$
$$f''''(x) = e^{x}$$

Evaluating the formula at $x=0$, we get

$$f(x) = e^{x}$$
$$= \sum_{n=0}^{\infty} \frac{f^{(n)}(0)}{n!}x^{n}$$
$$= f(0) + f'(0)x + f''(0)\frac{x^{2}}{2!} + f'''(0)\frac{x^{3}}{3!} + \cdots$$
$$= 1 + x + \frac{1}{2!}x^{2} + \frac{1}{3!}x^{3} + \frac{1}{4!}x^{4} + \cdots $$
$$= \sum_{n=0}^{\infty} \frac{x^{n}}{n!}$$


## Q3

$$f(x) = ln(1+x)$$

Taking derivatives, we have

$$f'(x) = (1+x)^{-1}$$
$$f''(x) = -(1+x)^{-2}$$
$$f'''(x) = 2(1+x)^{-3}$$
$$f''''(x) = -6(1+x)^{-4}$$

Evaluating the formula at $x=0$, we get

$$f(x) = ln(1+x)$$

$$= \sum_{n=0}^{\infty} \frac{f^{(n)}(0)}{n!}x^{n}$$
$$= f(0) + f'(0)x + f''(0)\frac{x^{2}}{2!} + f'''(0)\frac{x^{3}}{3!} + \cdots$$

$$= 0 + (0!)x + \frac{-1!}{2!}x^{2} + \frac{2!}{3!}x^{3} + \frac{-3!}{4!}x^{4} + \cdots $$
$$= 0 + \sum_{n=1}^{\infty} \frac{(-1)^{n-1}(n-1)!x^{n}}{n!}$$
$$= \sum_{n=1}^{\infty} \frac{(-1)^{n-1}x^{n}}{n}$$